src/Std/Tactic/BVDecide/LRAT/Internal/Formula/RupAddSound.lean
@@ -135,7 +135,7 @@ theorem sat_of_insertRup {n : Nat} (f : DefaultFormula n) (f_readyForRupAdd : Re
     simp only [Fin.getElem_fin, ne_eq, true_and, Bool.not_eq_true, exists_and_right]
     apply Or.inl
     intro j
-    simp only [f_readyForRupAdd.1, Array.size_toArray, List.length_nil] at j
+    simp only [f_readyForRupAdd.1, List.size_toArray, List.length_nil] at j
     exact Fin.elim0 j
   have insertUnit_fold_satisfies_invariant := insertUnitInvariant_insertUnit_fold f.assignments f_readyForRupAdd.2.1 f.rupUnits
     f.assignments f_readyForRupAdd.2.1 false (negate c) h0
@@ -157,7 +157,7 @@ theorem sat_of_insertRup {n : Nat} (f : DefaultFormula n) (f_readyForRupAdd : Re
       apply List.get_mem
     have ib_in_insertUnit_fold := mem_insertUnit_fold_units f.rupUnits f.assignments false (negate c) (i, b) ib_in_insertUnit_fold
     simp only [negate, Literal.negate, List.mem_map, Prod.mk.injEq, Prod.exists, Bool.exists_bool,
-      Bool.not_false, Bool.not_true, f_readyForRupAdd.1, Array.toList_toArray, List.find?, List.not_mem_nil, or_false]
+      Bool.not_false, Bool.not_true, f_readyForRupAdd.1, List.toList_toArray, List.find?, List.not_mem_nil, or_false]
       at ib_in_insertUnit_fold
     rw [hboth] at h2
     rcases ib_in_insertUnit_fold with ⟨i', ⟨i_false_in_c, i'_eq_i, b_eq_true⟩ | ⟨i_true_in_c, i'_eq_i, b_eq_false⟩⟩
@@ -211,7 +211,7 @@ theorem sat_of_insertRup {n : Nat} (f : DefaultFormula n) (f_readyForRupAdd : Re
     have i_false_in_insertUnit_fold :=
       mem_insertUnit_fold_units #[] f.assignments false (c.clause.map Literal.negate) (i, false) i_false_in_insertUnit_fold
     simp only [Literal.negate, List.mem_map, Prod.mk.injEq, Bool.not_eq_true', Prod.exists,
-      exists_eq_right_right, exists_eq_right, Array.toList_toArray, List.find?, List.not_mem_nil, or_false,
+      exists_eq_right_right, exists_eq_right, List.toList_toArray, List.find?, List.not_mem_nil, or_false,
       Bool.not_eq_false'] at i_true_in_insertUnit_fold i_false_in_insertUnit_fold
     have c_not_tautology := Clause.not_tautology c (i, true)
     simp only [Clause.toList, (· ⊨ ·)] at c_not_tautology
@@ -252,7 +252,7 @@ theorem assignmentsInvariant_insertRupUnits_of_assignmentsInvariant {n : Nat} (f
     rcases cf with cf | cf | cf
     · specialize hp c (Or.inl cf)
       exact hp
-    · simp only [f_readyForRupAdd.1, Array.toList_toArray, List.find?, List.not_mem_nil, false_and, or_self, exists_false] at cf
+    · simp only [f_readyForRupAdd.1, List.toList_toArray, List.find?, List.not_mem_nil, false_and, or_self, exists_false] at cf
     · specialize hp c <| (Or.inr ∘ Or.inr) cf
       exact hp
   rcases h ⟨i.1, i.2.2⟩ with ⟨h1, h2⟩ | ⟨j, b', i_gt_zero, h1, h2, h3, h4⟩ | ⟨j1, j2, i_gt_zero, h1, h2, _, _, _⟩
